---
hero:
  title: "Understanding Derivatives"
  subtitle: "The Foundation of Neural Network Training"
  tags:
    - "ğŸ“ Mathematics"
    - "â±ï¸ 10 min read"
---

[video coming soon]

What are Derivatives?

A derivative measures how a function changes as its input changes.

Intuitive Understanding

Think of driving a car:





Your position is a function of time: position(t)



Your speed is the derivative of position: speed = d(position)/dt



Speed tells you how fast your position is changing

If x goes from 3 to 4, does f(x), that is y, change fast, eg. 6 to 40 or slower, eg. 6 to 7

Derivative tells us the instantaneous rate of change of a function at any point.

Mathematical Definition

The derivative of f(x) at point x is:

f'(x) = lim[hâ†’0] (f(x+h) - f(x)) / h

Visual Representation



Here we have linearly growing function.

Derivative is always 3 for any x value, which means that in the original function, growth of y at any point is 3x (if you increase x by 1, y will increase by 3, check it).





Here you can see that as y grows faster and faster in original function (square functions grow very fast).

Derivative shows this accelerating growth, you can notice that derivative is increasing (linearly) - which means the growth is accelerating.

In previous example derivative was always 3, which meant that function is always consistantly growing by 3 times x.

Here, on the other hand, the growth is growing. 

Common Derivative Rules

You will never calculate derivatives manually, but researcher needs to understand how it works.

1. Power Rule

If f(x) = xâ¿, then f'(x) = nxâ¿â»Â¹

So just put the exponent in front of the variable (or multiply with the number in front) and reduce exponent by 1.

For f(x) = xÂ³, derivative is f'(x) = 3xÂ²

For f(x) = 4xÂ³, derivative is f'(x) = 4*3xÂ² = 12xÂ²

Step-by-Step Examples

Example 1: f(x) = xÂ²





Using power rule: f'(x) = 2x^(2-1) = 2xÂ¹ = 2x



Verification: f'(x) = 2x

Example 2: f(x) = xÂ³





Using power rule: f'(x) = 3x^(3-1) = 3xÂ²



Verification: f'(x) = 3xÂ²

Example 3: f(x) = xâ´





Using power rule: f'(x) = 4x^(4-1) = 4xÂ³



Verification: f'(x) = 4xÂ³

Example 4: f(x) = âˆšx = x^(1/2)





Using power rule: f'(x) = (1/2)x^((1/2)-1) = (1/2)x^(-1/2) = 1/(2âˆšx)



Verification: f'(x) = 1/(2âˆšx)

Example 5: f(x) = 1/x = x^(-1)





Using power rule: f'(x) = (-1)x^(-1-1) = (-1)x^(-2) = -1/xÂ²



Verification: f'(x) = -1/xÂ²



2. Constant Multiple Rule

If f(x) = cÂ·g(x), then f'(x) = cÂ·g'(x)

Step-by-Step Examples

Example: f(x) = 5xÂ²

Step 1: Identify the constant and the function





Constant: c = 5



Function: g(x) = xÂ²

Step 2: Find g'(x)





g'(x) = 2x (using power rule)

Step 3: Apply constant multiple rule





f'(x) = cÂ·g'(x) = 5Â·(2x) = 10x - I showed this in the power rule as well.

Verification:





f(x) = 5xÂ²



f'(x) = 10x âœ“

Example: f(x) = -3xÂ³

Step 1: Identify the constant and the function





Constant: c = -3



Function: g(x) = xÂ³

Step 2: Find g'(x)





g'(x) = 3xÂ² (using power rule)

Step 3: Apply constant multiple rule





f'(x) = cÂ·g'(x) = (-3)Â·(3xÂ²) = -9xÂ²

Verification:





f(x) = -3xÂ³



f'(x) = -9xÂ² âœ“



3. Sum Rule

If f(x) = g(x) + h(x), then f'(x) = g'(x) + h'(x)

Step-by-Step Examples

Example: f(x) = xÂ² + 3x

Step 1: Identify the functions





g(x) = xÂ²



h(x) = 3x

Step 2: Find individual derivatives





g'(x) = 2x (power rule)



h'(x) = 3 (constant multiple rule: 3Â·1 = 3)

Step 3: Apply sum rule





f'(x) = g'(x) + h'(x) = 2x + 3

Verification:





f(x) = xÂ² + 3x



f'(x) = 2x + 3 âœ“

Example: f(x) = xÂ³ + 2xÂ² + 5x + 1

Step 1: Identify the functions





g(x) = xÂ³



h(x) = 2xÂ²



i(x) = 5x



j(x) = 1

Step 2: Find individual derivatives





g'(x) = 3xÂ² (power rule)



h'(x) = 4x (constant multiple rule: 2Â·2x = 4x)



i'(x) = 5 (constant multiple rule: 5Â·1 = 5)



j'(x) = 0 (constant rule)

Step 3: Apply sum rule





f'(x) = g'(x) + h'(x) + i'(x) + j'(x) = 3xÂ² + 4x + 5 + 0 = 3xÂ² + 4x + 5

Verification:





f(x) = xÂ³ + 2xÂ² + 5x + 1



f'(x) = 3xÂ² + 4x + 5 âœ“



4. Product Rule

If f(x) = g(x)Â·h(x), then f'(x) = g'(x)Â·h(x) + g(x)Â·h'(x)

Step-by-Step Examples

Example: f(x) = xÂ²(x + 1)

Step 1: Identify the functions





g(x) = xÂ²



h(x) = x + 1

Step 2: Find individual derivatives





g'(x) = 2x (power rule)



h'(x) = 1 (sum rule: derivative of x is 1, derivative of 1 is 0)

Step 3: Apply product rule





f'(x) = g'(x)Â·h(x) + g(x)Â·h'(x)



f'(x) = (2x)Â·(x + 1) + (xÂ²)Â·(1)



f'(x) = 2x(x + 1) + xÂ²



f'(x) = 2xÂ² + 2x + xÂ²



f'(x) = 3xÂ² + 2x

Verification by expanding first:





f(x) = xÂ²(x + 1) = xÂ³ + xÂ²



f'(x) = 3xÂ² + 2x âœ“

Example: f(x) = (2x + 3)(xÂ² - 1)

Step 1: Identify the functions





g(x) = 2x + 3



h(x) = xÂ² - 1

Step 2: Find individual derivatives





g'(x) = 2 (sum rule: derivative of 2x is 2, derivative of 3 is 0)



h'(x) = 2x (sum rule: derivative of xÂ² is 2x, derivative of -1 is 0)

Step 3: Apply product rule





f'(x) = g'(x)Â·h(x) + g(x)Â·h'(x)



f'(x) = (2)Â·(xÂ² - 1) + (2x + 3)Â·(2x)



f'(x) = 2(xÂ² - 1) + (2x + 3)(2x)



f'(x) = 2xÂ² - 2 + 4xÂ² + 6x



f'(x) = 6xÂ² + 6x - 2



5. Chain Rule

If f(x) = g(h(x)), then f'(x) = g'(h(x))Â·h'(x)

Step-by-Step Examples

Example: f(x) = (xÂ² + 1)Â³

Step 1: Identify the inner and outer functions





Inner function: h(x) = xÂ² + 1



Outer function: g(u) = uÂ³ (where u = h(x))

Step 2: Find individual derivatives





h'(x) = 2x (sum rule: derivative of xÂ² is 2x, derivative of 1 is 0)



g'(u) = 3uÂ² (power rule)

Step 3: Apply chain rule





f'(x) = g'(h(x))Â·h'(x)



f'(x) = 3(h(x))Â²Â·(2x)



f'(x) = 3(xÂ² + 1)Â²Â·(2x)



f'(x) = 6x(xÂ² + 1)Â²

Verification by expanding first:





f(x) = (xÂ² + 1)Â³ = (xÂ² + 1)(xÂ² + 1)(xÂ² + 1)



Expanding: f(x) = xâ¶ + 3xâ´ + 3xÂ² + 1



f'(x) = 6xâµ + 12xÂ³ + 6x = 6x(xâ´ + 2xÂ² + 1) = 6x(xÂ² + 1)Â² âœ“

Example: f(x) = âˆš(xÂ² + 4)

Step 1: Identify the inner and outer functions





Inner function: h(x) = xÂ² + 4



Outer function: g(u) = âˆšu = u^(1/2) (where u = h(x))

Step 2: Find individual derivatives





h'(x) = 2x (sum rule: derivative of xÂ² is 2x, derivative of 4 is 0)



g'(u) = (1/2)u^(-1/2) = 1/(2âˆšu) (power rule)

Step 3: Apply chain rule





f'(x) = g'(h(x))Â·h'(x)



f'(x) = (1/(2âˆš(xÂ² + 4)))Â·(2x)



f'(x) = 2x/(2âˆš(xÂ² + 4))



f'(x) = x/âˆš(xÂ² + 4)



Derivatives of Neural Network Functions

1. Sigmoid Function





f(x) = 1 / (1 + e^(-x))

Step-by-Step Derivative Calculation

To find the derivative of sigmoid, we'll use the quotient rule and chain rule.

Usually you will ChatGPT sigmoid derivative, but let's see how it's derived.

Step 1: Rewrite the function





f(x) = 1 / (1 + e^(-x))



Let u = 1 + e^(-x), so f(x) = 1/u

Step 2: Apply quotient rule





f'(x) = (0Â·u - 1Â·u') / uÂ² = -u' / uÂ²

Step 3: Find u' using chain rule





u = 1 + e^(-x)



u' = 0 + e^(-x) Â· (-1) = -e^(-x)

Step 4: Substitute back





f'(x) = -(-e^(-x)) / (1 + e^(-x))Â²



f'(x) = e^(-x) / (1 + e^(-x))Â²

Step 5: Simplify





f'(x) = e^(-x) / (1 + e^(-x))Â²



f'(x) = [e^(-x) / (1 + e^(-x))] Â· [1 / (1 + e^(-x))]



f'(x) = [1 / (1 + e^(-x))] Â· [e^(-x) / (1 + e^(-x))]



f'(x) = f(x) Â· [e^(-x) / (1 + e^(-x))]

Step 6: Further simplification





Notice that e^(-x) / (1 + e^(-x)) = 1 - 1/(1 + e^(-x)) = 1 - f(x)



Therefore: f'(x) = f(x) Â· (1 - f(x))

Final Result: f'(x) = f(x)(1 - f(x))



Chain Rule

Chain rule is how neural networks learn (backpropagation).

Mathematical Statement

If y = f(g(x)), then dy/dx = (dy/dg) Ã— (dg/dx)

Neural Network Application

In neural networks, we often have functions like: f(x) = activation(linear_transformation(x))

Step-by-Step Chain Rule Example

Example: Neural Network Layer with Sigmoid Activation

Given:





Linear transformation: z = 2x + 1



Activation function: Ïƒ(z) = 1/(1 + e^(-z))



Composite function: f(x) = Ïƒ(2x + 1)

Step 1: Identify inner and outer functions





Inner function: h(x) = 2x + 1



Outer function: g(z) = Ïƒ(z) = 1/(1 + e^(-z))

Step 2: Find individual derivatives





h'(x) = 2 (derivative of 2x + 1)



g'(z) = Ïƒ(z)(1 - Ïƒ(z)) (sigmoid derivative)

Step 3: Apply chain rule





f'(x) = g'(h(x)) Â· h'(x)



f'(x) = Ïƒ(2x + 1)(1 - Ïƒ(2x + 1)) Â· 2



f'(x) = 2Ïƒ(2x + 1)(1 - Ïƒ(2x + 1))

Step 4: Calculate at specific point (x = 1)

Step 4a: Calculate h(1)





h(1) = 2(1) + 1 = 3

Step 4b: Calculate Ïƒ(3)





Ïƒ(3) = 1/(1 + e^(-3)) = 1/(1 + 0.050) = 1/1.050 â‰ˆ 0.953

Step 4c: Calculate Ïƒ'(3)





Ïƒ'(3) = Ïƒ(3)(1 - Ïƒ(3)) = 0.953(1 - 0.953) = 0.953(0.047) â‰ˆ 0.045

Step 4d: Apply chain rule





f'(1) = Ïƒ'(3) Â· h'(1) = 0.045 Â· 2 = 0.090

Final Answer: f'(1) â‰ˆ 0.090



Partial Derivatives

When we have functions of multiple variables, we use partial derivatives.

Definition

For f(x, y), the partial derivative with respect to x is: âˆ‚f/âˆ‚x = lim[hâ†’0] (f(x+h, y) - f(x, y)) / h

Example: Linear Function

f(x, y) = 2x + 3y + 1

Step-by-Step Partial Derivative Calculation

Finding âˆ‚f/âˆ‚x (partial derivative with respect to x):

Step 1: Treat y as a constant





f(x, y) = 2x + 3y + 1



When taking âˆ‚f/âˆ‚x, we treat y as constant, so 3y + 1 is constant

Step 2: Differentiate with respect to x





âˆ‚f/âˆ‚x = âˆ‚/âˆ‚x(2x) + âˆ‚/âˆ‚x(3y) + âˆ‚/âˆ‚x(1)



âˆ‚f/âˆ‚x = 2 + 0 + 0 = 2

Finding âˆ‚f/âˆ‚y (partial derivative with respect to y):

Step 1: Treat x as a constant





f(x, y) = 2x + 3y + 1



When taking âˆ‚f/âˆ‚y, we treat x as constant, so 2x + 1 is constant

Step 2: Differentiate with respect to y





âˆ‚f/âˆ‚y = âˆ‚/âˆ‚y(2x) + âˆ‚/âˆ‚y(3y) + âˆ‚/âˆ‚y(1)



âˆ‚f/âˆ‚y = 0 + 3 + 0 = 3

Final Results:





âˆ‚f/âˆ‚x = 2



âˆ‚f/âˆ‚y = 3

Hand Calculation Examples

Example: Find partial derivatives at (x, y) = (1, 2)





âˆ‚f/âˆ‚x = 2 (constant, doesn't depend on x or y)



âˆ‚f/âˆ‚y = 3 (constant, doesn't depend on x or y)

Example: Find partial derivatives at (x, y) = (5, -1)





âˆ‚f/âˆ‚x = 2 (still constant)



âˆ‚f/âˆ‚y = 3 (still constant)



Example: Quadratic Function

f(x, y) = xÂ² + 2xy + yÂ²

Step-by-Step Partial Derivative Calculation

Finding âˆ‚f/âˆ‚x (partial derivative with respect to x):

Step 1: Treat y as a constant





f(x, y) = xÂ² + 2xy + yÂ²



When taking âˆ‚f/âˆ‚x, we treat y as constant

Step 2: Differentiate with respect to x





âˆ‚f/âˆ‚x = âˆ‚/âˆ‚x(xÂ²) + âˆ‚/âˆ‚x(2xy) + âˆ‚/âˆ‚x(yÂ²)



âˆ‚f/âˆ‚x = 2x + 2y + 0 = 2x + 2y

Finding âˆ‚f/âˆ‚y (partial derivative with respect to y):

Step 1: Treat x as a constant





f(x, y) = xÂ² + 2xy + yÂ²



When taking âˆ‚f/âˆ‚y, we treat x as constant

Step 2: Differentiate with respect to y





âˆ‚f/âˆ‚y = âˆ‚/âˆ‚y(xÂ²) + âˆ‚/âˆ‚y(2xy) + âˆ‚/âˆ‚y(yÂ²)



âˆ‚f/âˆ‚y = 0 + 2x + 2y = 2x + 2y

Final Results:





âˆ‚f/âˆ‚x = 2x + 2y



âˆ‚f/âˆ‚y = 2x + 2y

Hand Calculation Examples

Example: Find partial derivatives at (x, y) = (1, 2)

Step 1: Calculate âˆ‚f/âˆ‚x





âˆ‚f/âˆ‚x = 2(1) + 2(2) = 2 + 4 = 6

Step 2: Calculate âˆ‚f/âˆ‚y





âˆ‚f/âˆ‚y = 2(1) + 2(2) = 2 + 4 = 6

Example: Find partial derivatives at (x, y) = (3, -1)

Step 1: Calculate âˆ‚f/âˆ‚x





âˆ‚f/âˆ‚x = 2(3) + 2(-1) = 6 - 2 = 4

Step 2: Calculate âˆ‚f/âˆ‚y





âˆ‚f/âˆ‚y = 2(3) + 2(-1) = 6 - 2 = 4